src/lowparse/LowParse.SteelST.Write.fst
@@ -1,0 +1,93 @@
+module LowParse.SteelST.Write
+module AP = LowParse.SteelST.ArrayPtr
+module SZ = LowParse.Steel.StdInt
+
+open Steel.ST.GenElim
+
+include LowParse.SteelST.Parse
+
+inline_for_extraction
+let writer
+  (#k: parser_kind)
+  (#t: Type)
+  (#p: parser k t)
+  (s: serializer p)
+: Tot Type
+=
+  (#va: _) ->
+  (x: t) ->
+  (a: byte_array) ->
+  ST SZ.size_t
+    (AP.arrayptr a va)
+    (fun sz -> exists_ (fun vl -> aparse p a vl `star` exists_ (fun ar -> exists_ (fun vr -> AP.arrayptr ar vr `star` pure (
+      AP.merge_into (array_of' vl) (AP.array_of vr) (AP.array_of va) /\
+      vl.contents == x /\
+      SZ.size_v sz == AP.length (array_of' vl)
+    )))))
+    (Seq.length (serialize s x) <= AP.length (AP.array_of va) /\
+      AP.array_perm (AP.array_of va) == full_perm)
+    (fun _ -> True)
+
+inline_for_extraction
+let exact_writer
+  (#k: parser_kind)
+  (#t: Type)
+  (#p: parser k t)
+  (s: serializer p)
+: Tot Type
+=
+  (#va: _) ->
+  (x: t) ->
+  (a: byte_array) ->
+  ST (v k t)
+    (AP.arrayptr a va)
+    (fun va' -> aparse p a va')
+    (Seq.length (serialize s x) == AP.length (AP.array_of va) /\
+      AP.array_perm (AP.array_of va) == full_perm)
+    (fun va' ->
+      array_of' va' == AP.array_of va /\
+      va'.contents == x
+    )
+
+inline_for_extraction
+let exact_write
+  (#k: parser_kind)
+  (#t: Type)
+  (#p: parser k t)
+  (#s: serializer p)
+  (w: writer s)
+: Tot (exact_writer s)
+= fun x a ->
+  let _ = w x a in
+  let _ = gen_elim () in
+  let va0 = elim_aparse _ a in
+  parse_injective p (AP.contents_of va0) (serialize s x);
+  let va1 = AP.join a _ in
+  assert (AP.contents_of va1 `Seq.equal` AP.contents_of va0);
+  let va' = intro_aparse p a in
+  return va'
+
+#push-options "--z3rlimit 16"
+#restart-solver
+
+inline_for_extraction
+let write_constant_size
+  (#k: parser_kind)
+  (#t: Type)
+  (#p: parser k t)
+  (#s: serializer p)
+  (w: exact_writer s)
+  (sz: SZ.size_t)
+: Pure (writer s)
+    (requires (
+      k.parser_kind_high == Some k.parser_kind_low /\
+      k.parser_kind_low == SZ.size_v sz
+    ))
+    (ensures (fun _ -> True))
+= fun x a ->
+  let ar = AP.split a sz in
+  let _ = gen_elim () in
+  let _ = w x a in
+  return sz
+
+#pop-options
